\paragraph{Exercise 1.7}
\begin{enumerate}
  \item[(a)] \textbf{Lemma 1.3} (\textcolor{WildStrawberry}{Inclusion-exclusion
    principle}): Let $E_1,...,E_n$ be any $n$ events. Then
    \[
      \pr\left(\bigcup_{i=1}^n E_i\right)
      = \sum_{i=1}^n \pr(E_i) - \sum_{i<j}\pr(E_i \cap E_j) + \sum_{i<j<k}\pr(E_i \cap E_j \cap E_k) - ... + (-1)^{l+1} \sum_{i_1<i_2< ... <i_l} \pr\left(\bigcap_{r=1}^lE_{i_r}\right)+ ... .
    \]
    \textit{Proof}. We want to show the Inclusion-exclusion principle by induction
    over $n \in \mathbb{N}$, where $n \geq 2$. \\
    For the base case (IB) assume that $n = 2$. According to Lemma 1.1, one has
    \begin{align*}
      \pr\left(E_1 \cup E_2 \right)
        &= \pr(E_1) + \pr(E_2) - \pr\left(E_1 \cap E_2 \right) \\
        &= \sum_{i=1}^2 \pr(E_i) - \sum_{i<j}\pr\left(E_1 \cap E_2 \right).
    \end{align*}
    Let $n \geq 2$, so that the Inclusion-exclusion principle holds for $n$
    (induction hypothesis, IH). We have to show, that the Inclusion-exclusion
    principle then also hold for $n+1$.
    \begin{align*}
      \pr\left(\bigcup_{i=1}^{n+1} E_i\right)
        &= \pr\left(\left(\bigcup_{i=1}^{n} E_i\right) \cup E_{n+1}\right) \\
        &=_{\text{Lemma 1.1}} \pr\left(\bigcup_{i=1}^{n} E_i\right) + \pr(E_{n+1}) -
            \pr\left(\left(\bigcup_{i=1}^{n} E_i\right) \cap E_{n+1}\right) \\
        &= \pr\left(\bigcup_{i=1}^{n} E_i\right) + \pr(E_{n+1}) -
            \pr\left(\bigcup_{i=1}^{n} \left(E_i \cap E_{n+1}\right)\right) \\
        &=_{IH} \pr(E_{n+1}) +
          \left(
            \sum_{i=1}^n \pr(E_i) - \sum_{i<j}\pr(E_i \cap E_j) + ... + (-1)^{n+1}
            \sum_{i_1<i_2< ... <i_n} \pr\left(\bigcap_{r=1}^n E_{i_r}\right)
          \right) \\
        &\ \ - \Bigg(
            \sum_{i=1}^n \pr\left(E_i \cap E_{n+1}\right) -
            \sum_{i<j} \pr\left((E_i \cap E_{n+1}) \cap (E_j \cap E_{n+1})\right)
            + ... \\
        &\quad \quad \quad+ (-1)^{n+1} \sum_{i_1<i_2< ... <i_n} \pr\left(\bigcap_{r=1}^n
            \left(E_{i_r} \cap E_{n+1}\right)\right)
          \Bigg) \\
        &= \sum_{i=1}^{n+1} \pr(E_i) - \sum_{i<j}\pr(E_i \cap E_j) + ... +
          (-1)^{n+1} \sum_{i_1<i_2< ... <i_n} \pr\left(\bigcap_{r=1}^n E_{i_r}\right) \\
        &\ \ - \Bigg(
            \sum_{i=1}^n \pr\left(E_i \cap E_{n+1}\right) - \sum_{i<j}\pr\left(E_i
            \cap E_j \cap E_{n+1}\right) + ...
         + (-1)^{n+1} \sum_{i_1<i_2< ... <i_n} \pr\left(\bigcap_{r=1}^n
          \left(E_{i_r} \cap E_{n+1}\right)\right)
          \Bigg) \\
        &= \sum_{i=1}^{n+1} \pr(E_i) - \sum_{i<j}\pr(E_i \cap E_j) +  ... + (-1)^{n+2}
          \sum_{i_1<i_2< ... <i_{n+1}} \pr\left(\bigcap_{r=1}^{n+1}E_{i_r}\right).
    \end{align*}
    Hence, the Inclusion-exclusion principle applies.

  \item[(b)] \textbf{Lemma 1.8}: Let $E_1,...,E_n$ be any $n$ events and $l \in
  \mathbb{N}$, so that $l$ is odd. Then
  \[
    \pr\left(\bigcup_{i=1}^n E_i\right)
    \leq \sum_{i=1}^n \pr(E_i) - \sum_{i<j}\pr(E_i \cap E_j) + \sum_{i<j<k}\pr(E_i \cap E_j \cap E_k) - ... + (-1)^{l+1} \sum_{i_1<i_2< ... <i_l} \pr\left(\bigcap_{r=1}^lE_{i_r}\right).
  \]
  \textit{Proof}. Let $l \in \mathbb{N}$, so that $3 \leq l \leq n$ and $l$ is odd. According to Lemma 1.3 one has,
  \begin{align*}
  \begin{tabular}{l}
    $\pr\left(\bigcup_{i=1}^n E_i\right) -
    \left(
      (-1)^{l+2} \sum_{i_1<i_2< ... <i_{l+1}} \pr\left(\bigcap_{r=1}^{l+1} E_{i_r}\right) + ... +
      (-1)^{n+1} \pr\left(\bigcap_{i=1}^n E_{i}\right)
    \right)$ \\
    $\ \ = \sum_{i=1}^n \pr(E_i) + ... + (-1)^{l+1} \sum_{i_1<i_2< ... <i_l}
      \pr\left(\bigcap_{r=1}^lE_{i_r}\right).$
  \end{tabular}
  \end{align*}
  Therefore, we have to show that
  \[
    (-1)^{l+2} \sum_{i_1<i_2< ... <i_{l+1}} \pr\left(\bigcap_{r=1}^{l+1} E_{i_r}\right)
    + ... + (-1)^{n+1} \pr\left(\bigcap_{i=1}^n E_{i}\right) \leq 0.
  \]
  Since $l$ is odd,
  \begin{align*}
      &(-1)^{l+2} \sum_{i_1<i_2< ... <i_{l+1}} \pr\left(\bigcap_{r=1}^{l+1} E_{i_r}\right) + ... + (-1)^{n+1} \pr\left(\bigcap_{i=1}^n E_{i}\right) \\
    = &-\sum_{i_1<i_2< ... <i_{l+1}} \pr\left(\bigcap_{r=1}^{l+1} E_{i_r}\right)
      + ... + (-1)^{n+1} \pr\left(\bigcap_{i=1}^n E_{i}\right).
  \end{align*}
  Furthermore, for any $1 \leq k < n$ holds,
  \[
    \sum_{i_1<i_2< ... <i_k} \pr\left(\bigcap_{r=1}^k E_{i_r}\right)
    \geq \sum_{i_1<i_2< ... <i_{k+1}} \pr\left(\bigcap_{r=1}^{k+1} E_{i_r}\right).
  \]
  Hence, for any pair $(k,k+1)$, there $l+1 \leq k < n$ and $k$ is even, holds
  \begin{align*}
    \   &(-1)^{k+1} \sum_{i_1<i_2< ... <i_{k}} \pr\left(\bigcap_{r=1}^{l+1} E_{i_r}\right) + (-1)^{k+2} \pr\left( \bigcap_{r=1}^{k+1} E_{i} \right) \\
    =   &-\sum_{i_1<i_2< ... <i_k} \pr\left( \bigcap_{r=1}^{l+1} E_{i_r} \right) + \pr\left(\bigcap_{r=1}^{k+1} E_{i}\right) \\
    \leq &\ 0.
  \end{align*}
  Therefore,
  \[
    (-1)^{l+2} \sum_{i_1<i_2< ... <i_{l+1}} \pr\left(\bigcap_{r=1}^{l+1} E_{i_r}\right)
    + ... + (-1)^{n+1} \pr\left(\bigcap_{i=1}^n E_{i}\right) \leq 0,
  \]
  and
  \[
    \pr\left(\bigcup_{i=1}^n E_i\right)
    \leq \sum_{i=1}^n \pr(E_i) - \sum_{i<j}\pr(E_i \cap E_j) + \sum_{i<j<k}\pr(E_i \cap E_j \cap E_k) - ... + (-1)^{l+1} \sum_{i_1<i_2< ... <i_l} \pr\left(\bigcap_{r=1}^lE_{i_r}\right).
  \]

  \item[(c)] \textbf{Lemma 1.9}: Let $E_1,...,E_n$ be any $n$ events and $l \in
  \mathbb{N}$, so that $l$ is even. Then
  \[
    \pr\left(\bigcup_{i=1}^n E_i\right)
    \geq \sum_{i=1}^n \pr(E_i) - \sum_{i<j}\pr(E_i \cap E_j) + \sum_{i<j<k}\pr(E_i \cap E_j \cap E_k) - ... + (-1)^{l+1} \sum_{i_1<i_2< ... <i_l} \pr\left(\bigcap_{r=1}^lE_{i_r}\right).
  \]
  \textit{Proof}. Let $l \in \mathbb{N}$, so that $2 \leq l \leq n$ and $l$ is even. Similarly to exercise 1.7b) we want now to show that
  \[
    (-1)^{l+2} \sum_{i_1<i_2< ... <i_{l+1}} \pr\left(\bigcap_{r=1}^{l+1} E_{i_r}\right)
    + ... + (-1)^{n+1} \pr\left(\bigcap_{i=1}^n E_{i}\right) \geq 0.
  \]
  Since $l$ is even,
  \begin{align*}
      &(-1)^{l+2} \sum_{i_1<i_2< ... <i_{l+1}} \pr\left(\bigcap_{r=1}^{l+1} E_{i_r}\right) + ... + (-1)^{n+1} \pr\left(\bigcap_{i=1}^n E_{i}\right) \\
    = &\sum_{i_1<i_2< ... <i_{l+1}} \pr\left(\bigcap_{r=1}^{l+1} E_{i_r}\right)
      - ... + (-1)^{n+1} \pr\left(\bigcap_{i=1}^n E_{i}\right).
  \end{align*}
  For any pair $(k,k+1)$, there $l+1 \leq k < n$ and $k$ is odd, holds
  \begin{align*}
    \   &(-1)^{k+1} \sum_{i_1<i_2< ... <i_{k}} \pr\left(\bigcap_{r=1}^{l+1} E_{i_r}\right) + (-1)^{k+2} \pr\left( \bigcap_{r=1}^{k+1} E_{i} \right) \\
    =   &\sum_{i_1<i_2< ... <i_k} \pr\left( \bigcap_{r=1}^{l+1} E_{i_r} \right) - \pr\left(\bigcap_{r=1}^{k+1} E_{i}\right) \\
    \geq &\ 0.
  \end{align*}
  Therefore,
  \[
    (-1)^{l+2} \sum_{i_1<i_2< ... <i_{l+1}} \pr\left(\bigcap_{r=1}^{l+1} E_{i_r}\right)
    + ... + (-1)^{n+1} \pr\left(\bigcap_{i=1}^n E_{i}\right) \geq 0,
  \]
  and
  \[
    \pr\left(\bigcup_{i=1}^n E_i\right)
    \geq \sum_{i=1}^n \pr(E_i) - \sum_{i<j}\pr(E_i \cap E_j) + \sum_{i<j<k}\pr(E_i \cap E_j \cap E_k) - ... + (-1)^{l+1} \sum_{i_1<i_2< ... <i_l} \pr\left(\bigcap_{r=1}^lE_{i_r}\right).
  \]

\end{enumerate}
