\textbf{Exercise 1.4}: Let us play a tournament in which we stop as soon as one
of us wins n games. We are evenly matched, so each of us wins any game with 
probability $\frac{1}{2}$, independently of other games. What is the probability 
that the loser has won $k$ games when the match is over? \\[0.2cm]
Let $X$ be the number of games the loser has won. We are interested in the 
probability that $X = k$, that is the probability that the tournament ends 
after $n + k$ games. Therefore, the winner has to win $n-1$ games among the first 
$n + k - 1$ games and additionally has to win the $(n+k)$-th game. Every tournament 
that fulfills this condition has probability $\frac{1}{2}^n \cdot \frac{1}{2}^{k}$. 
Since there are $\binom{n+k-1}{n-1}$ possibilities to choose $n-1$ games the winner 
wins among $n+k-1$ games,
\[
  \pr\left(X = k\right)
    = \binom{n+k-1}{n-1} \cdot \left(\frac{1}{2}\right)^n \cdot \left(\frac{1}{2}\right)^{k}
    = \binom{n+k-1}{n-1} \cdot \frac{1}{2^{n+k}}.
\]
To verify this result, we show that the following equation holds.
\[
  \sum_{k=0}^{n-1}\pr\left(X=k\right) = 1.
\]
Because of the symmetry of the binomial coefficient, that is $\binom{b}{a} = \binom{b}{b - a}$,
\begin{align*}
  \sum_{k=0}^{n-1}\pr\left(X=k\right)
    &= \sum_{k=0}^{n-1} \binom{n+k-1}{n-1} \cdot \frac{1}{2^n} \cdot \frac{1}{2^k} \\
    &= \sum_{k=0}^{n-1} \binom{n+k-1}{k} \cdot \frac{1}{2^n} \cdot \frac{1}{2^k} \\
    &= \frac{1}{2^n} \cdot \sum_{k=0}^{n-1} \binom{n+k-1}{k} \cdot \frac{1}{2^k}.
\end{align*}
Since $\binom{b}{a} = (-1)^a \binom{a - b - 1}{a}$,
\begin{align*}
  \sum_{k=0}^{n-1}\pr\left(X=k\right)
    &= \frac{1}{2^n} \cdot \sum_{k=0}^{n-1} \binom{n+k-1}{k} \cdot \frac{1}{2^k} \\
    &= \frac{1}{2^n} \cdot \sum_{k=0}^{n-1} \binom{k+n-1}{k} \cdot (-1)^k \left(- \frac{1}{2}\right)^{k} \\
    &= \frac{1}{2^n} \cdot \sum_{k=0}^{n-1} \binom{-n}{k} \cdot \left(- \frac{1}{2}\right)^{k}.
\end{align*}
Under consideration of the binomial series $(1 + x)^b = \sum_{a=0}^{\infty} \binom{b}{a}x^a, 
\quad |x| < 1, b \in \mathbb{R}$, we finally get
\begin{align*}
  \sum_{k=0}^{n-1}\pr\left(X=k\right)
    &= \frac{1}{2^n} \cdot \sum_{k=0}^{n-1} \binom{-n}{k} \cdot \left(- \frac{1}{2}\right)^{k} \\
    &= \frac{1}{2^n} \cdot \left(1 - \frac{1}{2}\right)^{-n} \\
    &= \frac{1}{2^n} \cdot 2^n \\
    &= 1.
\end{align*}
